src/program_proof/tulip/program/backup/start.v
@@ -1,0 +1,150 @@
+From Perennial.program_proof.tulip.program Require Import prelude.
+(* FIXME: adhoc fix to name collision, fix a global import in program prelude *)
+From Goose.github_com.mit_pdos.tulip Require Export backup.
+From Perennial.program_proof.tulip.program.backup Require Import
+  btcoord_repr bgcoord_repr start_bgcoord.
+
+Section program.
+  Context `{!heapGS Σ, !tulip_ghostG Σ}.
+
+  Theorem wp_Start
+    (tsW : u64) (rkW : u64) (cid : coordid) (ptgsP : Slice.t)
+    (gaddrmPP : loc) (gaddrmP : gmap u64 loc) (leader : u64) (proph : proph_id)
+    (ptgs : txnptgs) (gaddrm : gmap u64 (gmap u64 chan)) γ :
+    let ts := uint.nat tsW in
+    let rk := uint.nat rkW in
+    (1 < rk)%nat ->
+    dom gaddrm = gids_all ->
+    map_Forall (λ _ addrm, dom addrm = rids_all) gaddrm ->
+    safe_backup_txn γ ts ptgs -∗
+    is_txnptgs_in_slice ptgsP ptgs -∗
+    own_map gaddrmPP DfracDiscarded gaddrmP -∗
+    ([∗ map] addrmP; addrm ∈ gaddrmP; gaddrm, own_map addrmP DfracDiscarded addrm) -∗
+    know_tulip_inv_with_proph γ proph -∗
+    ([∗ map] gid ↦ addrm ∈ gaddrm, know_tulip_network_inv γ gid addrm) -∗
+    {{{ ([∗ set] gid ∈ gids_all, own_replica_backup_token γ cid.1 cid.2 ts rk gid) }}}
+      Start #tsW #rkW (coordid_to_val cid) (to_val ptgsP) #gaddrmPP #leader #proph
+    {{{ (tcoord : loc), RET #tcoord; own_backup_tcoord tcoord ts γ }}}.
+  Proof.
+    iIntros (ts rk Hrk Hgids Hrids) "#Hsafebk #Hptgs #HgaddrmP #Hgaddrm #Hinv #Hinvnets".
+    iIntros (Φ) "!> Htokens HΦ".
+    wp_rec.
+
+    (*@ func Start(ts, rank uint64, cid tulip.CoordID, ptgs []uint64, gaddrm tulip.AddressMaps, leader uint64, proph primitive.ProphId) *BackupTxnCoordinator { @*)
+    (*@     gcoords := make(map[uint64]*BackupGroupCoordinator)                 @*)
+    (*@                                                                         @*)
+    wp_apply (wp_NewMap).
+    iIntros (gcoordsPP) "HgcoordsP".
+
+    (*@     // Create a backup group coordinator for each participant group.    @*)
+    (*@     for _, gid := range(ptgs) {                                         @*)
+    (*@         addrm := gaddrm[gid]                                            @*)
+    (*@         gcoord := startBackupGroupCoordinator(addrm, cid, ts, rank)     @*)
+    (*@         gcoords[gid] = gcoord                                           @*)
+    (*@     }                                                                   @*)
+    (*@                                                                         @*)
+    iNamed "Hsafebk".
+    iDestruct "Hptgs" as (ptgsL) "(#HptgsL & %HptgsL & %Hnd)".
+    set P := (λ (i : u64),
+                ∃ (gcoords : gmap u64 loc),
+                  "HgcoordsP" ∷ own_map gcoordsPP (DfracOwn 1) gcoords ∗
+                  "Hgcoords" ∷ ([∗ map] gid ↦ gcoord ∈ gcoords,
+                                  is_backup_gcoord gcoord rk ts gid γ) ∗
+                  "Htks" ∷ ([∗ set] gid ∈ list_to_set (drop (uint.nat i) ptgsL),
+                              own_replica_backup_token γ cid.1 cid.2 ts rk gid) ∗
+                  "%Hdomgc" ∷ ⌜dom gcoords = list_to_set (take (uint.nat i) ptgsL)⌝)%I.
+    iMod (readonly_load with "HptgsL") as (q) "HptgsR".
+    iDestruct (own_slice_small_sz with "HptgsR") as %Hlenptgs.
+    wp_apply (wp_forSlice P with "[] [$HptgsR $HgcoordsP Htokens]"); last first; first 1 last.
+    { rewrite uint_nat_W64_0 drop_0 take_0 HptgsL dom_empty_L /=.
+      iSplit; first by iApply big_sepM_empty.
+      iSplit; last done.
+      iApply (big_sepS_subseteq with "Htokens").
+      rewrite Hvptgs.
+      apply subseteq_ptgroups.
+    }
+    { clear Φ.
+      iIntros (i gid Φ) "!> (HP & %Hinbound & %Hgid) HΦ".
+      iNamed "HP".
+      wp_pures.
+      wp_apply (wp_MapGet with "HgaddrmP").
+      iIntros (addrmP ok) "[%Hok HaddrmP]".
+      wp_pures.
+      assert (Hinptgs : gid ∈ ptgs).
+      { apply elem_of_list_lookup_2 in Hgid.
+        clear -Hgid HptgsL.
+        set_solver.
+      }
+      assert (Hin : gid ∈ gids_all).
+      { pose proof (subseteq_ptgroups (dom wrs)) as Hdom.
+        rewrite -Hvptgs in Hdom.
+        clear -Hdom Hinptgs.
+        set_solver.
+      }
+      iDestruct (big_sepM2_dom with "Hgaddrm") as %Hdomeq.
+      destruct ok; last first.
+      { exfalso.
+        apply map_get_false in Hok as [Hnotin _].
+        by rewrite -not_elem_of_dom Hdomeq Hgids in Hnotin.
+      }
+      apply map_get_true in Hok.
+      assert (is_Some (gaddrm !! gid)) as [addrm Haddrm].
+      { by rewrite -elem_of_dom -Hdomeq elem_of_dom. }
+      rewrite (drop_S _ _ _ Hgid) list_to_set_cons big_sepS_insert; last first.
+      { rewrite not_elem_of_list_to_set. intros Hgidin.
+        clear -Hgid Hgidin Hnd.
+        rewrite -(take_drop_middle _ _ _ Hgid) in Hnd.
+        apply NoDup_app in Hnd as (_ & _ & Hnd).
+        by apply NoDup_cons in Hnd as [? _].
+      }
+      iDestruct "Htks" as "[Htk Htks]".
+      wp_apply (wp_startBackupGroupCoordinator with "[] [$Hinv] [] Htk").
+      { apply Hrk. }
+      { apply Hin. }
+      { specialize (Hrids _ _ Haddrm). apply Hrids. }
+      { iApply (big_sepM2_lookup with "Hgaddrm").
+        { apply Hok. }
+        { apply Haddrm. }
+      }
+      { iApply (big_sepM_lookup with "Hinvnets"); first apply Haddrm. }
+      iIntros (gcoord) "Hgcoord".
+      wp_apply (wp_MapInsert with "HgcoordsP"); first done.
+      iIntros "HgcoordsP".
+      iApply "HΦ".
+      iFrame "HgcoordsP".
+      iSplitL "Hgcoords Hgcoord".
+      { iApply (big_sepM_insert_2 with "[Hgcoord] Hgcoords").
+        by iFrame "Hgcoord".
+      }
+      rewrite uint_nat_word_add_S; last word.
+      iFrame "Htks".
+      iPureIntro.
+      rewrite dom_insert_L.
+      rewrite (take_S_r _ _ _ Hgid) list_to_set_app_L Hdomgc /=.
+      clear.
+      set_solver.
+    }
+    iIntros "[HP _]".
+    iNamed "HP".
+    rewrite -Hlenptgs firstn_all HptgsL in Hdomgc.
+
+    (*@     tcoord := &BackupTxnCoordinator{                                    @*)
+    (*@         ts      : ts,                                                   @*)
+    (*@         rank    : rank,                                                 @*)
+    (*@         ptgs    : ptgs,                                                 @*)
+    (*@         gcoords : gcoords,                                              @*)
+    (*@         proph   : proph,                                                @*)
+    (*@     }                                                                   @*)
+    (*@     return tcoord                                                       @*)
+    (*@ }                                                                       @*)
+    wp_apply (wp_allocStruct).
+    { by auto 10. }
+    iIntros (gcoord) "Hgcoord".
+    iDestruct (struct_fields_split with "Hgcoord") as "Hgcoord".
+    iNamed "Hgcoord".
+    wp_pures.
+    iApply "HΦ".
+    by iFrame "∗ # %".
+  Qed.
+
+End program.
